P4SpecTec.lean
@@ -54,6 +54,7 @@ import P4SpecTec.Prelude.Iter
 import P4SpecTec.Prelude.Num
 import P4SpecTec.Prelude.Value
 import P4SpecTec.Refine.Calc
+import P4SpecTec.Refine.Init
 import P4SpecTec.Refine.StateCalc
 import P4SpecTec.Refine.StateRules
 import P4SpecTec.Refine.StateInterp
